\documentclass[12pt]{article}
\usepackage{amsmath,amssymb,amsfonts}
\usepackage[utf8]{inputenc}
\usepackage{geometry}
\geometry{a4paper, margin=1in}
\begin{document}

(8) $g(x) = \sin x^2 + \cos^2 x = \sin(x^2) + (\cos x)^2$
\begin{align*}
g'(x) &= \cos x^2 \cdot 2x + 2\cos x \cdot (-\sin x)
\end{align*}

(9) $g(x) = \tan(\cos x)$
\begin{align*}
g'(x) &= \sec^2(\cos x)(\cos x)' \\
&= \sec^2(\cos x)(-\sin x)
\end{align*}

(10) $g(x) = \tan x \cos x$
\begin{align*}
g'(x) &= (\tan x)'\cos x + \tan x(\cos x)' \\
&= \sec^2 x \cos x + \tan x(-\sin x)
\end{align*}

(11) $G(t) = e^{7t \sin 2t}$
\begin{align*}
G'(t) &= e^{7t \sin 2t} \cdot (7t \sin 2t)' \\
&= e^{7t \sin 2t} (7 \sin 2t + 7t \cos 2t \cdot 2)
\end{align*}

(12) $h(t) = \left(\frac{t^4+5}{t^2+5}\right)^3$
\begin{align*}
h'(t) &= 3\left(\frac{t^4+5}{t^2+5}\right)^2 \left(\frac{t^4+5}{t^2+5}\right)' \\
&= 3\left(\frac{t^4+5}{t^2+5}\right)^2 \left(\frac{4t^3(t^2+5) - (t^4+5)2t}{(t^2+5)^2}\right)
\end{align*}

(13) $y = \sin^2(\cos 3x) = (\sin(\cos 3x))^2$
% [Diagram: Chain rule decomposition x -> 3x -> Cos 3x -> Sin(Cos 3x) -> (Sin(Cos 3x))^2]
\begin{align*}
y' &= 2 \sin(\cos 3x) (\sin(\cos 3x))' \\
&= 2 \sin(\cos 3x) \cos(\cos 3x) (\cos 3x)' \\
&= 2 \sin(\cos 3x) \cos(\cos 3x) (-\sin 3x) (3x)' \\
&= 2 \sin(\cos 3x) \cos(\cos 3x) (-\sin 3x) \cdot 3
\end{align*}

\end{document}